Adds both list and single step spec Gallina signaling counter
- Also adds a simpler single step semantics

arrow-examples/SignalingCounter.v
@@ -63,6 +63,74 @@ Lemma arrow_and_expr_counter_semantics_agree:
   (map Bv2N (interp_sequential ((counter : Kappa _ _) _) signaling_counter_tb_inputs)).
 Proof. vm_compute; reflexivity. Qed.
 
+Lemma expr_single_step_agree:
+  (map Bv2N signaling_counter_tb_expected_outputs) =
+  (map Bv2N (interp_sequential11 ((counter : Kappa _ _) _) signaling_counter_tb_inputs)).
+Proof. vm_compute; reflexivity. Qed.
+
+Definition bv_add s (av bv: Bvector.Bvector s) :=
+    let a := Ndigits.Bv2N av in
+    let b := Ndigits.Bv2N bv in
+    let c := (a + b)%N in
+    (Ndigits.N2Bv_sized s c).
+
+(* List based specification *)
+Definition gallina_counter (inputs: list (bool * Bvector.Bvector 4)): list (Bvector.Bvector 4) :=
+  let zero := N2Bv_sized _ 0 in
+  rev (snd (fold_left (fun '(s, os) '(is_valid, value) =>
+    let last := hd zero os in
+      (if is_valid : bool then value else zero, bv_add _ last s :: os)) inputs (zero, []) )).
+
+Lemma spec_and_kappa_agree_on_given:
+  (map Bv2N (interp_sequential ((counter : Kappa _ _) _) signaling_counter_tb_inputs)) =
+  (map Bv2N (gallina_counter signaling_counter_tb_inputs)).
+Proof. vm_compute; reflexivity. Qed.
+
+Lemma kappa_counter_is_gallina_counter: forall is,
+  gallina_counter is =
+  interp_sequential ((counter : Kappa _ _) _) is.
+Proof.
+  intros.
+  induction is; [auto|].
+  (* This goal should be true, otherwise bug in spec/semantics*)
+  (* gallina_counter (a :: is) = interp_sequential (counter list_func) (a :: is) *)
+Admitted.
+
+Notation state := (list {k & denote_kind k}).
+
+(* Single step specification *)
+Definition gallina_counter_single_step1
+  (s: state) (inputs : bool * Bvector.Bvector 4): (state * Bvector.Bvector 4) :=
+  let '(is_valid, value) := inputs in
+  let inc := if is_valid then value else N2Bv_sized _ 0 in
+  let s := match s with
+           | [] => N2Bv_sized _ 0
+           | existT _ sk s :: _ => ArrowKind.rewrite_or_default sk (Vector Bit 4) s
+           end in
+  ([existT _ (Vector Bit 4) (bv_add _ s inc)], s).
+
+Lemma singlestep_agree_on_a_point:
+  interp_sequential1 ((counter : Kappa _ _) _) [] (true, N2Bv_sized _ 1) =
+  gallina_counter_single_step1 [] (true, N2Bv_sized _ 1).
+Proof. vm_compute; reflexivity. Qed.
+
+Lemma kappa_counter_is_gallina_counter_single_step: forall is,
+  gallina_counter_single_step1 [] is =
+  interp_sequential1 ((counter : Kappa _ _) _) [] is.
+Proof.
+  intros.
+  destruct is.
+  cbv [gallina_counter_single_step1
+    interp_sequential1 interp_sequential1' interp_combinational'
+    counter coq_func denote_apply_rightmost_tt denote_kind module_to_expr module_body
+    fst snd
+    mux_item enable KappaNotation.unsigned_add1 replicate map2 bitwise
+    primitive_output primitive_semantics binary_semantics unary_semantics nullary_semantics
+    app bv_add kind_default].
+
+  (* some vector expression that should be true*)
+Admitted.
+
 Definition signaling_counter_tb :=
   testBench "signaling_counter_tb" signaling_counter_Interface
             signaling_counter_tb_inputs signaling_counter_tb_expected_outputs.
